Compiler/Proofs/IRGeneration/GenericInduction.lean
@@ -5,6 +5,13 @@ import Compiler.Proofs.IRGeneration.FunctionBody
 import Compiler.Proofs.IRGeneration.IRInterpreter
 import Compiler.Proofs.IRGeneration.SupportedSpec
 
+set_option linter.unnecessarySeqFocus false
+set_option linter.unnecessarySimpa false
+set_option linter.unreachableTactic false
+set_option linter.unusedSimpArgs false
+set_option linter.unusedTactic false
+set_option linter.unusedVariables false
+
 namespace Compiler.Proofs.IRGeneration
 
 open Compiler
